aarch64 refine+crefine: GIC_v3 proof updates
- abstract over the value of max_armKSGICVCPUNumListRegs
- adjust virq access proofs
- abstract over vcpu type size in C (changes with GIC version, because
  number of LR registers changes)

Signed-off-by: Gerwin Klein <gerwin.klein@proofcraft.systems>

proof/refine/AARCH64/ArchInvsDefs_H.thy
@@ -216,7 +216,7 @@ definition valid_asid_table' :: "(asid \<rightharpoonup> machine_word) \<Rightar
 definition "is_vcpu' \<equiv> \<lambda>ko. \<exists>vcpu. ko = (KOArch (KOVCPU vcpu))"
 
 definition max_armKSGICVCPUNumListRegs :: nat where
-  "max_armKSGICVCPUNumListRegs \<equiv> 63"
+  "max_armKSGICVCPUNumListRegs \<equiv> if config_ARM_GIC_V3 then 16 else 64"
 
 definition valid_arch_state' :: "kernel_state \<Rightarrow> bool" where
   "valid_arch_state' \<equiv> \<lambda>s.
@@ -225,7 +225,7 @@ definition valid_arch_state' :: "kernel_state \<Rightarrow> bool" where
    (case armHSCurVCPU (ksArchState s) of
       Some (v, b) \<Rightarrow> ko_wp_at' (is_vcpu' and hyp_live') v s
       | _ \<Rightarrow> True) \<and>
-   armKSGICVCPUNumListRegs (ksArchState s) \<le> max_armKSGICVCPUNumListRegs \<and>
+   armKSGICVCPUNumListRegs (ksArchState s) < max_armKSGICVCPUNumListRegs \<and>
    canonical_address (addrFromKPPtr (armKSGlobalUserVSpace (ksArchState s)))"
 
 definition archMakeObjectT :: "arch_kernel_object_type \<Rightarrow> kernel_object" where
@@ -236,4 +236,8 @@ definition archMakeObjectT :: "arch_kernel_object_type \<Rightarrow> kernel_obje
       | VCPUT \<Rightarrow> injectKO (makeObject :: vcpu)"
 
 end
+
+(* Need to declare code equation outside Arch locale *)
+declare AARCH64.max_armKSGICVCPUNumListRegs_def[code]
+
 end
