proof/refine/AARCH64/Interrupt_R.thy
@@ -736,16 +736,6 @@ lemma dmo_gets_wp:
 crunch vgicUpdateLR
   for ksCurThread[wp]: "\<lambda>s. P (ksCurThread s)"
 
-lemma virqType_eq[simp]:
-  "virqType = virq_type"
-  unfolding virqType_def virq_type_def
-  by simp
-
-lemma virqSetEOIIRQEN_eq[simp]:
-  "AARCH64_H.virqSetEOIIRQEN = AARCH64_A.virqSetEOIIRQEN"
-  unfolding virqSetEOIIRQEN_def AARCH64_A.virqSetEOIIRQEN_def
-  by auto
-
 lemma not_pred_tcb':
   "(\<not>pred_tcb_at' proj P t s) = (\<not>tcb_at' t s \<or> pred_tcb_at' proj (\<lambda>a. \<not>P a) t s)"
   by (auto simp: pred_tcb_at'_def obj_at'_def)
